

# Supplementary Material for “An ADMM-based Battery Dispatch Optimization Approach for Electric Vehicle Aggregators with Input-Discriminative Local Differential Privacy Budgets”

Chao Lei, *Member, IEEE*, Qifeng Li, *Senior Member, IEEE*, Siqi Bu, *Senior Member, IEEE*, and Qianggang Wang, *Senior Member, IEEE*

## I. PROOF OF THEOREM 1

There exists an optimal BDO solution  $\mathbf{x}_i^{t*}$  with the minimum objective function value  $\mathbf{F}^*$  for the C-BDO model (1a)-(1d). We incorporate  $\mathbf{p}_{sig,i}^{t*} \in \mathbb{R}$  such that  $\sum_{i=1}^{N_E} \mathbf{p}_{sig,i}^{t*} = \mathbf{p}_{ref}^t$ . Reformulate  $\|\cdot\|_2$  in the objective function (1a) by

$$\left\| \sum_{i=1}^{N_E} \mathbf{c}^T \mathbf{x}_i^{t*} - \mathbf{p}_{ref}^t \right\|_2 = \left\| \sum_{i=1}^{N_E} (\mathbf{c}^T \mathbf{x}_i^{t*} - \mathbf{p}_{sig,i}^{t*}) \right\|_2 \quad (\text{I-1})$$

Then, we achieve optimality by

$$\sum_{t=1}^{N_T} \left\| \sum_{i=1}^{N_E} (\mathbf{c}^T \mathbf{x}_i^{t*} - \mathbf{p}_{sig,i}^{t*}) \right\|_2 = \sum_{t=1}^{N_T} \left\| \sum_{i=1}^{N_E} \mathbf{c}^T \mathbf{x}_i^{t*} - \mathbf{p}_{ref}^t \right\|_2 = \mathbf{F}^* \quad (\text{I-2})$$

This proves that  $(\mathbf{x}_i^{t*}, \mathbf{p}_{sig,i}^{t*}) \in \mathcal{X}$  can be the optimal BDO solution with the minimum objective function value  $\mathbf{F}^*$ .

Due to the triangle inequality of norms, i.e.,  $|a + b| \leq |a| + |b|$  for any real-valued numbers  $a$  and  $b$ , we obtain that  $\mathbf{F}^* \leq \mathbf{F} \leq \mathbf{G}$  naturally holds. This suggests that  $\mathbf{F}^*$  can be the lower bound of  $\mathbf{G}$  over  $\mathcal{X}$ . In other words,  $(\mathbf{x}_i^{t*}, \mathbf{p}_{sig,i}^{t*}) \in \mathcal{X}$  can be the optimal solution iff the minimum function value  $\mathbf{G}^* = \mathbf{F}^*$  is achieved, which demonstrates  $(\mathbf{x}_i^{t*}, \mathbf{p}_{sig,i}^{t*})$  can also be the optimal BDO solution for minimizing the objective function  $\mathbf{G}$  over the feasibility space  $\mathcal{X}$ . This proves Theorem 1. ■

## II. PROOF OF THEOREM 2

The objective is to prove that the optimal charge-discharge solution  $\mathbf{x}_i^{t\dagger} = \mathbf{x}_i^{t*}$  holds for EV<sub>*i*</sub>. It is clear that the following (II-3) stands.

$$\mathbf{s}_i^{t*} = \mathbf{c}^T \mathbf{x}_i^{t*} - \mathbf{p}_{sig,i}^{t*} + \alpha_i^{t\dagger} \xi_i^t - \alpha_i^{t\dagger} \xi_i^t. \quad (\text{II-3})$$

We denote  $\tilde{\mathbf{p}}_{sig,i}^{t\dagger} = \mathbf{p}_{sig,i}^{t*} + \alpha_i^{t\dagger} \xi_i^t$ . Then, we have

$$\mathbf{s}_i^{t*} = \mathbf{c}^T \mathbf{x}_i^{t*} - \tilde{\mathbf{p}}_{sig,i}^{t\dagger} + \alpha_i^{t\dagger} \xi_i^t \quad (\text{II-4})$$

As  $\mathbf{s}_i^{t\dagger} \geq \mathbf{s}_i^{t*}$  and  $\mathbf{y}_i^{t\dagger} = \mathbf{s}_i^{t\dagger}$  achieved at optimality, minimizing the objective function  $\mathbf{g}_i$  ensures  $\mathbf{s}_i^{t\dagger} = \mathbf{s}_i^{t*}$ , where other two terms in  $\mathbf{g}_i$  can be held at convergence, i.e.,

$$\mu^t (\tilde{\mathbf{p}}_{sig,i}^{t\dagger} - \alpha_i^{t\dagger} \xi_i^t) = \mu^t \mathbf{p}_{sig,i}^{t*} \quad (\text{II-5})$$

and

$$\frac{\phi}{2} \left\| \sum_{j=1, j \neq i}^{N_E} \tilde{\mathbf{p}}_{sig,j}^{t\dagger} + \tilde{\mathbf{p}}_{sig,i}^{t\dagger} - \mathbf{p}_{ref}^t \right\|_2^2 = \frac{\phi}{2} \left\| \sum_{j=1, j \neq i}^{N_E} \mathbf{p}_{sig,j}^{t*} + \mathbf{p}_{sig,i}^{t*} - \mathbf{p}_{ref}^t \right\|_2^2 \approx 0 \quad (\text{II-6})$$

Thus, we rewrite  $\mathbf{s}_i^{t\dagger} = \mathbf{c}^T \mathbf{x}_i^{t*} - \tilde{\mathbf{p}}_{sig,i}^{t\dagger} + \alpha_i^{t\dagger} \xi_i^t$ . This suggests that  $\mathbf{x}_i^{t\dagger} = \mathbf{x}_i^{t*}$  holds with obfuscated  $\tilde{\mathbf{p}}_{sig,i}^{t\dagger} = \mathbf{p}_{sig,i}^{t*} + \alpha_i^{t\dagger} \xi_i^t$  for the privacy-preserving BDO model. ■

## III. PROOF OF THEOREM 3

We prove that  $\mathcal{M}$  is  $r_{\epsilon,i}^t$ -ID-LDP with respect to the local dataset of sub-problem  $i$  during all iterations. Let the query output answer for the sub-problem  $i$  be  $\mathcal{O}_i^t = \tilde{\mathbf{p}}_{sig,i}^t$ , and we alternatively rewrite (III-7) in the definition of  $r_{\epsilon,i}^t$ -LDP for the sub-problem  $i$ :

$$\mathbb{P}[\mathcal{M}_i = \mathcal{O}_i^t | \mathbf{x}_i^t] \leq \mathbb{P}[\mathcal{M}_i = \mathcal{O}_i^t | \mathbf{x}_i^{t'}] e^{r_{\epsilon,i}^t}, \quad (\text{III-7})$$

for two  $r_{\epsilon,i}^t$ -indistinguishable charge-discharge solutions  $\mathbf{x}_i^t$  and  $\mathbf{x}_i^{t'}$  in time period  $t$ . For convenience, the query output  $\mathcal{O}_i^t$  of EV<sub>*i*</sub> for  $\forall t \in \mathcal{T}$  with a random noise  $\xi_i^t$  can be written as  $\mathcal{O}_i^t = \tilde{\mathbf{p}}_{sig,i}^t = \mathbf{p}_{sig,i}^t + \alpha_i^t \xi_i^t$  where  $\forall t \in \mathcal{T}$ .

Therefore, the ratio of probabilities on two  $\epsilon_i$ -indistinguishable charge-discharge solutions  $\mathbf{x}_i^t$  and  $\mathbf{x}_i^{t'}$  can be bounded by

$$\begin{aligned} \frac{\mathbb{P}[\mathcal{M}_i = \mathcal{O}_i^t | \mathbf{x}_i^t]}{\mathbb{P}[\mathcal{M}_i = \mathcal{O}_i^t | \mathbf{x}_i^{t'}]} &= \frac{\mathbb{P}[\mathbf{p}_{sig,i}^t + \alpha_i^t \xi_i^t = \mathcal{O}_i^t | \mathbf{x}_i^t]}{\mathbb{P}[\mathbf{p}_{sig,i}^{t'} + \alpha_i^t \xi_i^t = \mathcal{O}_i^t | \mathbf{x}_i^{t'}]} \\ &= \frac{\mathbb{P}[\alpha_i^t \xi_i^t = \mathcal{O}_i^t - \mathbf{p}_{sig,i}^t | \mathbf{x}_i^t]}{\mathbb{P}[\alpha_i^t \xi_i^t = \mathcal{O}_i^t - \mathbf{p}_{sig,i}^{t'} | \mathbf{x}_i^{t'}]} \stackrel{(i)}{=} \frac{\alpha_i^t \exp\left\{-\frac{r_{\epsilon,i}^t \|\mathcal{O}_i^t - \mathbf{p}_{sig,i}^t\|_1}{\Delta_{\rho,i}}\right\}}{\alpha_i^t \exp\left\{-\frac{r_{\epsilon,i}^t \|\mathcal{O}_i^t - \mathbf{p}_{sig,i}^{t'}\|_1}{\Delta_{\rho,i}}\right\}} \\ &= \exp\left(\frac{r_{\epsilon,i}^t \|\mathcal{O}_i^t - \mathbf{p}_{sig,i}^t\|_1 - r_{\epsilon,i}^t \|\mathcal{O}_i^t - \mathbf{p}_{sig,i}^{t'}\|_1}{\Delta_{\rho,i}}\right) \\ &\stackrel{(ii)}{\leq} \exp\left(\frac{r_{\epsilon,i}^t \|\mathbf{p}_{sig,i}^t - \mathbf{p}_{sig,i}^{t'}\|_1}{\Delta_{\rho,i}}\right) \stackrel{(iii)}{\leq} \exp\left(\frac{r_{\epsilon,i}^t \Delta_{\rho,i}}{\Delta_{\rho,i}}\right) = e^{r_{\epsilon,i}^t}, \end{aligned} \quad (\text{III-8})$$

where (i) comes from the definition of the probability density function of the Gaussian distribution. In (ii) step, it is followed by the inequality of norms, i.e.,  $|a| - |b| \leq |a - b|$  for any real-valued numbers  $a$  and  $b$ . For the (iii) step,  $\|\mathbf{p}_{sig,i}^t - \mathbf{p}_{sig,i}^{t'}\|_1$  denotes the  $\ell_1$ -sensitivity on  $\rho$ -indistinguishable output datasets  $\mathbf{p}_{sig,i}^t$  and  $\mathbf{p}_{sig,i}^{t'}$  subject to  $\|\mathbf{p}_{sig,i}^t - \mathbf{p}_{sig,i}^{t'}\|_1 \leq \Delta_{\rho,i}$ .

Accordingly, it is clear that (III-7) holds based on (III-8), which proves this Theorem. ■